src/Sound/Data/State/Model.dfy
@@ -7,8 +7,10 @@ module Model {
       Not, Equiv, Or, Negate, Plus, Minus, Times, Div, Mod, Less, 
       AtMost, NoEmptyTypes, InterpFunctionOn
     reveals Any, True, False, LogicAnd, IsBool, IsInt, HasType, Implies, 
-      Literal, FunctionSig, Function, Type, Int, Bool, 
+      Literal, FunctionSig, Function, Type, Int, Bool, Eql, Neql, IsBoolSet, IsIntSet,
       HaveTypes
+      ,BoolUnaryFunc, BoolBinaryFunc, IntUnaryFunc, IntBinaryFunc, BinaryFunc,
+      InterpretBoolUnaryFuncISet, InterpretBoolBinaryFuncISet, InterpretIntUnaryFuncISet, InterpretIntBinaryFuncISet, InterpretBinaryFuncISet
 
   type Type = string
   const Int : Type := "int"
@@ -16,8 +18,6 @@ module Model {
   datatype Literal = Literal(value: string, typ: Type)
   type FunctionSig = seq<Type>
   datatype Function = Function(name: string, sig: FunctionSig, resultType: Type)
-
-
 
   type Any(!new, ==)
 
@@ -43,6 +43,14 @@ module Model {
     HasType(x, Bool)
   }
 
+  ghost predicate IsBoolSet(xs: iset<Any>) {
+    forall x <- xs :: IsBool(x)
+  }
+
+  ghost predicate IsIntSet(xs: iset<Any>) {
+    forall x <- xs :: IsInt(x)
+  }
+
   function {:axiom} InterpInt(x: int): Any
     ensures HasType(InterpInt(x), Int)
 
@@ -60,6 +68,16 @@ module Model {
   const True: Any := InterpBool(true)
   const False: Any := InterpBool(false)
 
+  function Eql(x: Any, y: Any): Any
+  {
+    InterpBool(x == y)
+  }
+
+  function Neql(x: Any, y: Any): Any
+  {
+    InterpBool(x != y)
+  }
+
   function Not(x: Any): Any
     requires IsBool(x) 
   {
@@ -67,7 +85,7 @@ module Model {
   }
 
   function LogicAnd(x: Any, y: Any): Any
-    requires IsBool(x) 
+    requires IsBool(x)
     requires IsBool(y)
   {
     InterpBool(ToBool(x) && ToBool(y))
@@ -156,4 +174,59 @@ module Model {
   function {:axiom} InterpFunctionOn(func: Function, args: seq<Any>): Any
     requires HaveTypes(args, func.sig)
     ensures HasType(InterpFunctionOn(func, args), func.resultType)
+
+  // type BoolFunc = f: seq<Any> --> Any | forall ss: seq<Any> :: (forall s <- ss :: IsBool(s)) ==> f.requires(ss)
+  // type IntFunc = f: seq<Any> --> Any | forall ss: seq<Any> :: (forall s <- ss :: IsInt(s)) ==> f.requires(ss)
+  // type PolymorphicFunc = f: seq<Any> -> Any
+
+  function InterpretBinaryBoolFunc(f: BoolBinaryFunc, ss: seq<Any>): Any
+    requires forall s <- ss :: IsBool(s)
+  {
+    f(ss[0], ss[1])
+  }
+
+
+
+  type BinaryFunc = (Any, Any) -> Any
+  type BoolUnaryFunc = f: Any --> Any | forall x :: IsBool(x) ==> f.requires(x)
+    witness Not
+
+  type BoolBinaryFunc = f: (Any, Any) --> Any | forall x, y :: IsBool(x) && IsBool(y) == f.requires(x, y)
+    witness LogicAnd
+
+  type IntUnaryFunc = f: Any --> Any | forall x :: IsInt(x) ==> f.requires(x)
+    witness Negate
+
+  type IntBinaryFunc = f: (Any, Any) --> Any | forall x, y :: IsInt(x) && IsInt(y) ==> f.requires(x, y)
+    witness Plus
+
+  ghost predicate InterpretBinaryFuncISet(f: BinaryFunc, xs: iset<Any>, ys: iset<Any>, outs: iset<Any>) {
+    forall x <- xs, y <- ys :: f(x, y) in outs
+  }
+
+  ghost predicate InterpretBoolUnaryFuncISet(f: BoolUnaryFunc, xs: iset<Any>, outs: iset<Any>) 
+    requires forall x <- xs :: IsBool(x)
+  {
+    forall x <- xs :: f(x) in outs
+  }
+
+  ghost predicate InterpretBoolBinaryFuncISet(f: BoolBinaryFunc, xs: iset<Any>, ys: iset<Any>, outs: iset<Any>) 
+    requires forall x <- xs :: IsBool(x)
+    requires forall y <- ys :: IsBool(y)
+  {
+    forall x <- xs, y <- ys :: f(x, y) in outs
+  }
+
+  ghost predicate InterpretIntUnaryFuncISet(f: IntUnaryFunc, xs: iset<Any>, outs: iset<Any>) 
+    requires forall x <- xs :: IsInt(x)
+  {
+    forall x <- xs :: f(x) in outs
+  }
+
+  ghost predicate InterpretIntBinaryFuncISet(f: IntBinaryFunc, xs: iset<Any>, ys: iset<Any>, outs: iset<Any>) 
+    requires forall x <- xs :: IsInt(x)
+    requires forall y <- ys :: IsInt(y)
+  {
+    forall x <- xs, y <- ys :: f(x, y) in outs
+  }
 }
